Introduce two notions of reachability for context graphs

proofs/ContextGraph/ContextGraph.v
@@ -15,34 +15,66 @@ Section ContextGraph.
   Variable node : Set.
 
   (*
-    Context graphs are directed, i.e., every edge is associated with a source
-    node and a target node. Each edge is also labeled with another node which
-    is called its *context*. Every node induces a subgraph defined by the
-    subset of edges which have that node as their context together with any
-    nodes which are their endpoints. Here, edges are indicated by a predicate
-    parameterized by the context, source, and target, respectively.
-    Specializing the predicate on a particular context yields the binary edge
-    relation for the subgraph induced by that context.
+    Context graphs are directed, i.e., each edge is associated with a source
+    node and a target node. Each edge is also labeled with another node called
+    its *context*. Here, edges are indicated by a predicate on the context,
+    source, and target, respectively. Specializing the predicate on a
+    particular context yields a binary edge relation which induces a subgraph
+    for that context.
   *)
 
   Variable edge : node -> node -> node -> Prop.
 
   (*
-    A node is *rooted in* a context if it's reachable from that context in the
-    subgraph induced by that context. This predicate is used to define a well-
-    formedness condition below.
+    *Interior reachability* is the transitive reflexive closure of the edge
+    relation specialized on a particular context. Reflexivity is immediate from
+    the definition, and transitivity is proven below.
   *)
 
-  Inductive rooted (context : node) : node -> Prop :=
-  | loop :
-    rooted context context
-  | extension :
+  Inductive interiorReachable (context : node) (start : node) : node -> Prop :=
+  | interiorReflexivity :
+    interiorReachable context start start
+  | interiorExtension :
     forall source target,
-    rooted context source ->
+    interiorReachable context start source ->
     edge context source target ->
-    rooted context target.
+    interiorReachable context start target.
 
-  #[local] Hint Constructors rooted : main.
+  #[local] Hint Constructors interiorReachable : main.
+
+  (* Interior reachability contains the edge relation. *)
+
+  Theorem interiorReachableComplete :
+    forall context source target,
+    edge context source target ->
+    interiorReachable context source target.
+  Proof.
+    clean.
+    apply interiorExtension with (source := source); magic.
+  Qed.
+
+  (*
+    Interior reachability is reflexive by definition. Here, we show that it's
+    also transitive and thus a preorder.
+  *)
+
+  Theorem interiorTransitivity :
+    forall context node1 node2 node3,
+    interiorReachable context node1 node2 ->
+    interiorReachable context node2 node3 ->
+    interiorReachable context node1 node3.
+  Proof.
+    clean.
+    induction H0; magic.
+    apply interiorExtension with (source := source); magic.
+  Qed.
+
+  (*
+    A node is *rooted in* a context if it's interior reachable in and from that
+    context.
+  *)
+
+  Definition rooted context := interiorReachable context context.
 
   (*
     For a context graph to be *well-formed*, it must satisfy the following
@@ -55,8 +87,8 @@ Section ContextGraph.
     rooted context source.
 
   (*
-    The condition above immediately implies the following as a corollary: the
-    target of every edge is rooted in that edge's context.
+    The condition above immediately implies the following corollary: the target
+    of every edge is rooted in that edge's context.
   *)
 
   Theorem targetsRooted :
@@ -65,54 +97,63 @@ Section ContextGraph.
     rooted context target.
   Proof.
     clean.
-    apply extension with (source := source); magic.
+    apply interiorExtension with (source := source); magic.
     apply sourcesRooted with (target := target).
     magic.
   Qed.
 
   (*
-    A node is *accessible* from a context if it is that context or if it's
-    rooted in a nested context which is accessible from that context.
+    *Exterior reachability* is the transitive reflexive closure of the rooted
+    relation. Reflexivity is immediate from the definition, and transitivity is
+    proven below.
   *)
 
-  Inductive accessible (context : node) : node -> Prop :=
-  | identity :
-    accessible context context
-  | nested :
-    forall nestedContext node,
-    accessible context nestedContext ->
-    rooted nestedContext node ->
-    accessible context node.
+  Inductive exteriorReachable (start : node) : node -> Prop :=
+  | exteriorReflexivity :
+    exteriorReachable start start
+  | exteriorExtension :
+    forall context node,
+    exteriorReachable start context ->
+    rooted context node ->
+    exteriorReachable start node.
 
-  #[local] Hint Constructors accessible : main.
+  #[local] Hint Constructors exteriorReachable : main.
 
-  (* These two theorems establish that accessibility is a preorder. *)
+  (* Exterior reachability contains the rooted relation. *)
 
-  Theorem accessibleReflexive : forall node, accessible node node.
-  Proof.
-    magic.
-  Qed.
-
-  Theorem accessibleTransitive :
-    forall node1 node2 node3,
-    accessible node1 node2 ->
-    accessible node2 node3 ->
-    accessible node1 node3.
+  Theorem exteriorReachableComplete :
+    forall context node, rooted context node -> exteriorReachable context node.
   Proof.
     clean.
-    induction H0; magic.
-    apply nested with (nestedContext := nestedContext); magic.
+    apply exteriorExtension with (context := context); magic.
   Qed.
 
   (*
-    Since the nodes of the subgraph induced by a context must be rooted in that
-    context, one might also expect a similar situation for the graph as a
-    whole. Here we formalize that criterion by postulating the existence of a
-    global context from which every node is accessible.
+    Exterior reachability is reflexive by definition. Here, we show that it's
+    also transitive and thus a preorder.
+  *)
+
+  Theorem exteriorTransitivity :
+    forall node1 node2 node3,
+    exteriorReachable node1 node2 ->
+    exteriorReachable node2 node3 ->
+    exteriorReachable node1 node3.
+  Proof.
+    clean.
+    induction H0; magic.
+    apply exteriorExtension with (context := context); magic.
+  Qed.
+
+  (*
+    Since the nodes of the subgraph induced by the edges for a particular
+    context must be rooted in that context, one might also expect an analogous
+    situation for the graph as a whole. Here we formalize that criterion by
+    postulating the existence of an *origin* context from which every node is
+    exterior reachable.
   *)
 
   Variable origin : node.
 
-  Hypothesis originality : forall node, accessible origin node.
+  Hypothesis originality : forall node, exteriorReachable origin node.
 
 End ContextGraph.
